build.sh
@@ -1,0 +1,3 @@
+#!/bin/sh
+bash test.sh
+isabelle build -D Isabelle
